Bump Iris version
IPM broke the abstraction between seplog.derives and predicates_hered.derives, so this fixes it by wrapping it in an Inductive.

msl/alg_seplog.v
@@ -13,6 +13,18 @@ Require VST.msl.normalize.
 
 Local Open Scope logic.
 
+Inductive nd_derives {T: Type}{agT: ageable T} A B := { derivesI: predicates_hered.derives A B }.
+
+Lemma nd_derives_eq {T: Type}{agT: ageable T} : nd_derives = predicates_hered.derives(H := agT).
+Proof.
+  do 2 extensionality.
+  apply prop_ext; split.
+  - inversion 1; auto.
+  - constructor; auto.
+Qed.
+
+Ltac unseal_derives := intros; rewrite ?nd_derives_eq; repeat match goal with H : context[nd_derives] |- _ => rewrite nd_derives_eq in H; revert H end.
+
 Instance algNatDed (T: Type){agT: ageable T} : NatDed (pred T).
   apply (mkNatDed _
                     predicates_hered.andp
@@ -20,7 +32,7 @@ Instance algNatDed (T: Type){agT: ageable T} : NatDed (pred T).
                     (@predicates_hered.exp _ _)
                     (@predicates_hered.allp _ _)
                     predicates_hered.imp predicates_hered.prop
-                    (@predicates_hered.derives _ _)).
+                    (nd_derives)); unseal_derives.
  apply pred_ext.
  apply derives_refl.
  apply derives_trans.
@@ -30,10 +42,10 @@ Instance algNatDed (T: Type){agT: ageable T} : NatDed (pred T).
  apply orp_left.
  apply orp_right1.
  apply orp_right2.
- intros ? ?; apply @exp_right.
- intros ? ?; apply @exp_left.
- intros ? ?; apply @allp_left.
- intros ? ?; apply @allp_right.
+ apply @exp_right.
+ apply @exp_left.
+ apply @allp_left.
+ apply @allp_right.
  apply imp_andp_adjoint.
  repeat intro. eapply H; eauto. hnf; auto.
  repeat intro. hnf; auto.
@@ -44,7 +56,7 @@ Defined.
 Instance algSepLog (T: Type) {agT: ageable T}{JoinT: Join T}{PermT: Perm_alg T}{SepT: Sep_alg T}{AgeT: Age_alg T} :
       @SepLog (pred T) (algNatDed T).
  apply (mkSepLog _ (algNatDed T) predicates_sl.emp predicates_sl.sepcon
-            predicates_sl.wand predicates_sl.ewand).
+            predicates_sl.wand predicates_sl.ewand); simpl; unseal_derives.
  apply sepcon_assoc.
  apply sepcon_comm.
  intros. pose proof (wand_sepcon_adjoint P Q R). simpl. rewrite H; split; auto.
@@ -68,14 +80,14 @@ Instance TrivNatDed: NatDed Triv := algNatDed nat.
 Instance TrivSeplog: SepLog Triv := @algSepLog nat _ _ _ _ (asa_nat).
 Instance TrivClassical: ClassicalSep Triv := @algClassicalSep _ _ _ _ _ asa_nat.
 Instance TrivIntuitionistic: IntuitionisticSep Triv.
- constructor. intros. hnf. intros. destruct H as [w1 [w2 [? [? _]]]].
+ constructor. intros. hnf. constructor. hnf. intros. destruct H as [w1 [w2 [? [? _]]]].
  destruct H; subst; auto.
 Qed.
 
 Instance algIndir (T: Type) {agT: ageable T}{JoinT: Join T}{PermT: Perm_alg T}{SepT: Sep_alg T}
                 {AgeT: Age_alg T}:
          @Indir (pred T) (algNatDed T).
- apply (mkIndir _ _ (box laterM)); intros; simpl in *.
+ apply (mkIndir _ _ (box laterM)); intros; simpl in *; unseal_derives.
  apply @predicates_hered.now_later.
  apply @predicates_hered.axiomK.
  apply @predicates_hered.later_allp.
@@ -125,11 +137,11 @@ Notation "P '<=>' Q" := (# (P <--> Q)) (at level 57, no associativity) : logic.
 
 Definition algRecIndir (T: Type) {agT: ageable T}{JoinT: Join T}{PermT: Perm_alg T}{SepT: Sep_alg T}{AgeT: Age_alg T} :
          @RecIndir (pred T) (algNatDed T) (algIndir T).
- apply (mkRecIndir _ _ _ subtypes.fash subtypes.unfash HoRec.HORec); intros; simpl.
+ apply (mkRecIndir _ _ _ subtypes.fash subtypes.unfash HoRec.HORec); intros; simpl in *; unseal_derives.
  repeat intro. do 3 red in H. apply H; auto.
  apply @subtypes.fash_K.
  apply @subtypes.fash_derives; auto.
- intros ? ?. do 3 red in H0. apply H in H0. apply H0.
+ intros ? ?. do 3 red in H. apply H.
  apply @subtypes.later_fash; auto.
  apply @subtypes.later_unfash.
  apply @subtypes.fash_and.
@@ -149,7 +161,7 @@ Section SL3. Import VST.msl.seplog.
 Lemma fash_triv: forall P: Triv, fash P = P.
 Proof.
  intros.
- apply pred_ext; intros ? ?.
+ apply pred_ext; simpl; unseal_derives; intros ? ?.
  eapply H. unfold level; simpl.  unfold natLevel; auto.
  hnf; intros. eapply pred_nec_hereditary; try eapply H.
  apply nec_nat. auto.
