concurrency/semax_conc.v
@@ -54,7 +54,7 @@ Lemma nonexpansive_entail (F: pred rmap -> pred rmap) : nonexpansive F -> forall
 Proof.
   intros N P Q.
   specialize (N P Q).
-  eapply derives_trans; [ eapply derives_trans | ]; [ | apply N | ];
+  eapply derives_trans; [ eapply derives_trans | ]; [ | constructor; apply N | ];
   apply derives_refl.
 Qed.
 
@@ -65,11 +65,11 @@ Proof.
   + intros P Q.
     specialize (H (P tt) (Q tt)).
     rewrite !allp_unit.
-    auto.
+    constructor; auto.
   + intros P Q.
     specialize (H (fun x => P) (fun x => Q)).
     rewrite !allp_unit in H.
-    auto.
+    inv H; auto.
 Qed.
 
 Lemma selflock'_eq Q sh p : selflock' Q sh p =
@@ -79,7 +79,7 @@ Proof.
   intros P1 P2 u.
   apply subp_sepcon; [ apply subp_refl | ].
   rewrite <- subp_later.
-  repeat intro.
+  constructor; repeat intro.
   match goal with |- app_pred (?P >=> ?Q)%logic ?a => change (subtypes.fash (P --> Q) a) end.
   unfold lock_inv; repeat intro.
   destruct H3 as (b & ofs & ? & Hl & ?); exists b, ofs; split; auto; split; auto.
@@ -114,7 +114,9 @@ Lemma eqp_sepcon : forall (G : Triv) (P P' Q Q' : mpred)
 Proof.
   intros.
   rewrite fash_andp in HP, HQ |- *.
-  apply andp_right; apply subp_sepcon; auto; intros ? Ha; destruct (HP _ Ha), (HQ _ Ha); auto.
+  inv HP; rename derivesI into HP.
+  inv HQ; rename derivesI into HQ.
+  apply andp_right; apply subp_sepcon; auto; constructor; intros ? Ha; destruct (HP _ Ha), (HQ _ Ha); auto.
 Qed.
 
 Lemma eqp_andp : forall (G : Triv) (P P' Q Q' : mpred)
@@ -122,7 +124,9 @@ Lemma eqp_andp : forall (G : Triv) (P P' Q Q' : mpred)
 Proof.
   intros.
   rewrite fash_andp in HP, HQ |- *.
-  apply andp_right; apply subp_andp; auto; intros ? Ha; destruct (HP _ Ha), (HQ _ Ha); auto.
+  inv HP; rename derivesI into HP.
+  inv HQ; rename derivesI into HQ.
+  apply andp_right; apply subp_andp; auto; constructor; intros ? Ha; destruct (HP _ Ha), (HQ _ Ha); auto.
 Qed.
 
 Lemma eqp_exp : forall (A : Type) (NA : NatDed A) (IA : Indir A) (RecIndir : RecIndir A)
@@ -132,7 +136,7 @@ Lemma eqp_exp : forall (A : Type) (NA : NatDed A) (IA : Indir A) (RecIndir : Rec
 Proof.
   intros.
   rewrite fash_andp; apply andp_right; apply subp_exp; intro x; specialize (H x); rewrite fash_andp in H;
-    intros ? Ha; destruct (H _ Ha); auto.
+    inv H; rename derivesI into H; constructor; intros ? Ha; destruct (H _ Ha); auto.
 Qed.
 
 Lemma lock_inv_nonexpansive2 : forall {A} (P Q : A -> mpred) sh p x, (ALL x : _, |> (P x <=> Q x) |--
@@ -269,8 +273,7 @@ Proof.
   intros.
   apply approx_eq_i'.
   intros m ?.
-  pose proof nonexpansive_entail _ H R (approx n R) m.
-  apply H1.
+  apply nonexpansive_entail; auto.
   clear - H0.
   apply (fash_equiv_approx n R m); auto.
 Qed.
@@ -284,9 +287,11 @@ Proof.
   intros.
   apply approx_eq_i'.
   intros m ?.
-  pose proof nonexpansive_entail _ (H P) Q (approx n Q) m; cbv beta in H2.
+  pose proof nonexpansive_entail _ (H P) Q (approx n Q) as H2.
+  inv H2; rename derivesI into H2. specialize (H2 m); cbv beta in H2.
   spec H2; [apply (fash_equiv_approx n Q m); auto |].
-  pose proof nonexpansive_entail _ (H0 (approx n Q)) P (approx n P) m; cbv beta in H3.
+  pose proof nonexpansive_entail _ (H0 (approx n Q)) P (approx n P) as H3.
+  inv H3; rename derivesI into H3. specialize (H3 m); cbv beta in H3.
   spec H3; [apply (fash_equiv_approx n P m); auto |].
   remember (F P Q) as X1.
   remember (F P (approx n Q)) as X2.
